coq_new/sta_type.v
@@ -63,12 +63,12 @@ Inductive sta0_type : sta_ctx -> term -> term -> Prop :=
   sta0_type (Sig0 A B t :: Γ) C (Sort s) ->
   sta0_type Γ m (Sig0 A B t) ->
   sta0_type (B :: A :: Γ) n C.[Pair0 (Var 1) (Var 0) t .: ren (+2)] ->
-  sta0_type Γ (LetIn0 C m n) C.[m/]
+  sta0_type Γ (LetIn C m n) C.[m/]
 | sta0_letin1 Γ A B C m n s t :
   sta0_type (Sig1 A B t :: Γ) C (Sort s) ->
   sta0_type Γ m (Sig1 A B t) ->
   sta0_type (B :: A :: Γ) n C.[Pair1 (Var 1) (Var 0) t .: ren (+2)] ->
-  sta0_type Γ (LetIn1 C m n) C.[m/]
+  sta0_type Γ (LetIn C m n) C.[m/]
 | sta0_with Γ A B s r t :
   sta0_type Γ A (Sort s) ->
   sta0_type Γ B (Sort r) ->
@@ -76,7 +76,7 @@ Inductive sta0_type : sta_ctx -> term -> term -> Prop :=
 | sta0_apair Γ A B m n t :
   sta0_type Γ m A ->
   sta0_type Γ n B ->
-  sta0_type Γ (APair A B t) (With A B t)
+  sta0_type Γ (APair m n t) (With A B t)
 | sta0_fst Γ A B m t :
   sta0_type Γ m (With A B t) ->
   sta0_type Γ (Fst m) A
@@ -90,11 +90,11 @@ Inductive sta0_type : sta_ctx -> term -> term -> Prop :=
 | sta0_refl Γ A m :
   sta0_type Γ m A ->
   sta0_type Γ (Refl m) (Id A m m)
-| sta0_rew Γ A B H P m n s :
+| sta0_j Γ A B H P m n s :
   sta0_type (Id A.[ren (+2)] (Var 1) (Var 0) :: A.[ren (+1)] :: A :: Γ) B (Sort s) ->
   sta0_type (A :: Γ) H B.[Refl (Var 0) .: Var 0 .: Var 0 .: ren (+1)] ->
   sta0_type Γ P (Id A m n) ->
-  sta0_type Γ (Rew B H P) B.[P,n,m/]
+  sta0_type Γ (J B H P) B.[P,n,m/]
 | sta0_conv Γ A B m s :
   A === B ->
   sta0_type Γ m A ->
@@ -171,12 +171,12 @@ Inductive sta_type : sta_ctx -> term -> term -> Prop :=
   (Sig0 A B t :: Γ) ⊢ C : Sort s ->
   Γ ⊢ m : Sig0 A B t ->
   (B :: A :: Γ) ⊢ n : C.[Pair0 (Var 1) (Var 0) t .: ren (+2)] ->
-  Γ ⊢ LetIn0 C m n : C.[m/]
+  Γ ⊢ LetIn C m n : C.[m/]
 | sta_letin1 Γ A B C m n s t :
   (Sig1 A B t :: Γ) ⊢ C : Sort s ->
   Γ ⊢ m : Sig1 A B t ->
   (B :: A :: Γ) ⊢ n : C.[Pair1 (Var 1) (Var 0) t .: ren (+2)] ->
-  Γ ⊢ LetIn1 C m n : C.[m/]
+  Γ ⊢ LetIn C m n : C.[m/]
 | sta_with Γ A B s r t :
   Γ ⊢ A : Sort s ->
   Γ ⊢ B : Sort r ->
@@ -184,7 +184,7 @@ Inductive sta_type : sta_ctx -> term -> term -> Prop :=
 | sta_apair Γ A B m n t :
   Γ ⊢ m : A ->
   Γ ⊢ n : B ->
-  Γ ⊢ APair A B t : With A B t
+  Γ ⊢ APair m n t : With A B t
 | sta_fst Γ A B m t :
   Γ ⊢ m : With A B t ->
   Γ ⊢ Fst m : A
@@ -198,11 +198,11 @@ Inductive sta_type : sta_ctx -> term -> term -> Prop :=
 | sta_refl Γ A m :
   Γ ⊢ m : A ->
   Γ ⊢ Refl m : Id A m m
-| sta_rew Γ A B H P m n s :
+| sta_j Γ A B H P m n s :
   (Id A.[ren (+2)] (Var 1) (Var 0) :: A.[ren (+1)] :: A :: Γ) ⊢ B : Sort s ->
   (A :: Γ) ⊢ H : B.[Refl (Var 0) .: Var 0 .: Var 0 .: ren (+1)] ->
   Γ ⊢ P : Id A m n ->
-  Γ ⊢ Rew B H P : B.[P,n,m/]
+  Γ ⊢ J B H P : B.[P,n,m/]
 | sta_conv Γ A B m s :
   A === B ->
   Γ ⊢ m : A ->
